% !TeX root = ./TMA02.tex
\def\F{\mathcal{F\xspace}}%
\def\L{\left(}%
\def\R{\right)}%
\def\osu{\L\frac{1}{\sqrt{2}}\cdot u\R}%
Solving for the associated \el for the functional \eqref{eq:1.1}:
\[
	\textrm{Let}\quad \F = y^2 - 2y^{\prime2},
\]
then
\[
	\pderiv{\F}{y^\prime} = -4 y^\prime,
\]
\[
	\deriv{}{u}\L\pderiv{\F}{y^\prime}\R = \deriv{}{u}\L-4 y^\prime\R = -4 y^\dprime,
\]
\[
	\textrm{and}\quad \deriv{\F}{y} = 2 y.
\]
The \el is
\[
	-4\deriv{^2y}{u^2} - 2y = 0,
\]
which after dividing through by $-4$ becomes
\[
	\deriv{^2y}{u^2} +\half y = 0.
\]
The auxiliary equation for the above \el is
\[
	\lambda^2 + \half = 0, \quad \textrm{and the roots are} \quad \lambda_{1,2} = \pm i\frac{1}{\sqrt{2}}.
\]
Hence, the general solution is
\begin{equation}
\label{eq:1.2}
	y = c_1\cos\osu + c_2\sin\osu,
\end{equation}
where, $c_1$ and $c_2$ are arbitrary constants.