% !TeX root = ./TMA02.tex
\def\osx[#1]{{\L\frac{1}{\sqrt{2}}\cosh {#1}\R}}%
\def\os2{\frac{1}{\sqrt{2}}}%
Substituting into \eqref{eq:1.2} for $u=\cosh x$ gives,
\begin{equation}
\label{eq:1.4}
	y(x) = c_1\cos\osx[x] + c_2\sin\osx[x],
\end{equation}
Now, when $x=1$, $y=0$ and when $x=2$, $y=2$. Substituting  these boundary conditions into the above expression for $y$ \eqref{eq:1.4} gives the following pair of simultaneous equations,
\begin{align*}
	0 =& c_1\cos\osx[1] + c_2\sin\osx[1],\quad\textrm{and}\\
	2 =& c_1\cos\osx[2] + c_2\sin\osx[2].
\end{align*}
Solving for the constants $c_1$ and $c_2$ gives,
\begin{align*}
	c_1 =&\frac{
				-2\sin\osx[1]
		      }
		      {
		      	\sin\osx[2]\cos\osx[1]-\sin\osx[1]\cos\osx[2]
		      },\\
	c_2 =&\frac{
				2\cos\osx[1]
		      }
		      {
		      	\sin\osx[2]\cos\osx[1]-\sin\osx[1]\cos\osx[2]
		      }.      
\end{align*}
Making use of the identity $\sin\L\alpha-\beta\R = \sin\alpha\cos\beta -\cos\alpha\sin\beta$, then the above pair of equations can be simplified to
\begin{align*}
	c_1 =&\frac{
				-2\sin\osx[1]
		      }
		      {
		      	\sin \L \os2 \cosh 2 - \os2 \cosh 1\R
		      },\\
	c_2 =&\frac{
				2\cos\osx[1]
		      }
		      {
		      	\sin \L \os2 \cosh 2 - \os2 \cosh 1\R
		      }.      
\end{align*}
Thus, substituting into \eqref{eq:1.4} for $c_1$ and $c_2$ gives,
\[
	y(x) = \frac{
				-2\sin\osx[1]\cos\osx[x] + 2\cos\osx[1]\sin\osx[x]
			}
			{
				\sin \L \os2 \cosh 2 - \os2 \cosh 1\R
			}.
\]
Simplifying the above using the same trig identity as before gives,
\[
	y(x) = \frac{
				2\sin\L\os2\L\cosh x - \cosh 1\R \R
			}
			{
				\sin \L \os2 \cosh 2 - \os2 \cosh 1\R
			}
\]
as required.