% !TeX root = ./TMA02.tex
\def\yp{y^{\prime}}
\vspace{-6mm}
\begin{equation*}
	F=f(x)\,\,\sqrt[â€¢]{1+y^{\prime2}} = f(x)\,\,\lr{1 + y^{\prime2}}^\half.
\end{equation*}
The \el is,
\[
	\ELE{F}{x}{y},
\]
\[
	\deriv{}{x}\lr{\pderiv{F}{y^\prime}} = 0,\quad\textrm{so, }\quad\pderiv{F}{y^\prime} = \beta,\quad \textrm{where } \beta \textrm{ is a constant.}
\]
\[
	\pderiv{F}{y^\prime} =\half\, f(x) \lr{ 1+y^{\prime2}}^{-\half}\,2y^\prime = \beta.
\]
\begin{align*}
	f(x) \,   \frac{y^\prime}{\lr{1 + y^{\prime2}}^\half} =&\beta,\\
	f(x)^2 \, \frac{y^{\prime2}}{\lr{1 + y^{\prime2}}} =& \beta^2,\\
	f(x)^2 \,y^{\prime2} = \beta^2\lr{1 + y^{\prime2}} =& \beta^2 + \beta y^{\prime2},\\
	f(x)^2 \,y^{\prime2} - \beta^2 - \beta^2 y^{\prime2} =& 0,\\
	y^{\prime2} \,\lr{f(x)^2 - \beta^2 } =& \beta^2,\\
	y^{\prime2}  = \frac{\beta^2}{\lr{f(x)^2 - \beta^2 }}.\\
	\textrm{Thus,}\quad y^{\prime}  = \frac{\beta}{\sqrt{f(x)^2 - \beta^2 }}.
\end{align*}
Integrating the last expression gives,
\[
	y(x) = C + \beta \Int{a}{x}{w}\frac{1}{\sqrt{f(w)^2 - \beta^2 }},\quad\textrm{where $C$ is a constant.}
\]
Now, $y(a) = A$, and applying this to the above expression for $y(x)$ gives,
\[
	A = C + \cancelto{0}{\beta\int_a^a\dd w\, \frac{1}{\sqrt{f(w)^2 -\beta^2}}},\qquad\textrm{therefore, } C=A.
\]
\[
	\textrm{Hence,}\qquad y(x) = A + \beta \Int{a}{x}{w}\frac{1}{\sqrt{f(w)^2 - \beta^2 }},\qquad\textrm{as required.}
\]
Also, $y(b) = B$ so,
\[
	B = A + \beta\int_a^b\dd w\, \frac{1}{\sqrt{f(w)^2 -\beta^2}}.
\]
Hence, the constant $\beta$ satisfies,
\[
	B - A = \beta \int_a^b\dd w\, \frac{1}{\sqrt{f(w)^2 -\beta^2}}.
\]